src/coqutil/Map/OfFunc.v
@@ -1,0 +1,129 @@
+Require Import coqutil.Decidable coqutil.Map.Interface coqutil.Map.MapKeys.
+Require coqutil.Decidable coqutil.Map.Properties.
+Require Coq.Lists.List.
+Import MapKeys.map Interface.map.
+
+Module map.
+  Section OfFunc.
+    Context {key value} {map : map key value} {ok : map.ok map}.
+    Context {key_eqb: key -> key -> bool} {key_eq_dec: EqDecider key_eqb}.
+
+    Context (f : key -> option value).
+    Fixpoint of_func (support : list key) : map :=
+      match support with
+      | nil => empty
+      | cons k support => update (of_func support) k (f k)
+      end.
+
+    Lemma get_of_func_In k support (Hs : List.In k support)
+      : get (of_func support) k = f k.
+    Proof.
+      revert dependent support.
+      induction support.
+      { firstorder idtac. }
+      { destruct (key_eq_dec a k); intros [|]; subst;
+          pose proof Properties.map.get_update_same;
+          cbn; try congruence; [].
+        rewrite Properties.map.get_update_diff by congruence.
+        eauto. }
+    Qed.
+
+    Lemma get_of_func_Some_In k support v (H:get (of_func support) k = Some v)
+      : List.In k support.
+    Proof.
+      revert dependent support.
+      induction support.
+      { cbn. rewrite get_empty. discriminate. }
+      { destruct (key_eq_dec a k); subst; cbn [List.In of_func]; eauto.
+        rewrite Properties.map.get_update_diff by congruence; eauto. }
+    Qed.
+
+    Lemma get_of_func_notIn k support (Hs : not (List.In k support))
+      : get (of_func support) k = None.
+    Proof.
+      case (get (of_func support) k) eqn:H; trivial.
+      eapply get_of_func_Some_In in H; intuition.
+    Qed.
+
+    Lemma get_of_func_None k s (H:f k = None) : get (of_func s) k = None.
+    Proof.
+      induction s.
+      { firstorder idtac. }
+      { destruct (key_eq_dec a k); subst.
+        { cbn [of_func]. cbv [update].
+          rewrite H, get_remove_same; trivial. }
+        { cbn; rewrite Properties.map.get_update_diff; congruence. } }
+    Qed.
+
+    Lemma get_of_func_Some_supported_In
+      support (Hs : forall k v, f k = Some v -> List.In k support)
+      k v (Hk : f k = Some v)
+      : get (of_func support) k = f k.
+    Proof. eauto using get_of_func_In. Qed.
+
+    Lemma get_of_func_Some_supported
+      support (Hs : forall k v, f k = Some v -> List.In k support) k
+      : get (of_func support) k = f k.
+    Proof.
+      case (f k) eqn:H.
+      { pose proof get_of_func_Some_supported_In _ Hs _ _ H; congruence. }
+      { eauto using get_of_func_None. }
+    Qed.
+
+    Lemma get_of_func_type_supported k support (Hs : forall k, List.In k support) 
+      : get (of_func support) k = f k.
+    Proof. eauto using get_of_func_In. Qed.
+  End OfFunc.
+
+  Import Coq.Lists.List coqutil.Datatypes.List Interface.map.
+  Section OfListNatAt.
+    Context {value : Type} {map : map nat value} {ok : map.ok map}.
+    Definition of_list_nat (xs : list value) : map :=
+      of_func (nth_error xs) (seq 0 (length xs)).
+    Definition of_list_nat_at (a : nat) (xs : list value) : map :=
+      map_keys (Nat.add a) (of_list_nat xs).
+
+    Lemma get_of_list_nat xs i : get (of_list_nat xs) i = nth_error xs i.
+    Proof.
+      pose proof Nat.eqb_spec.
+      cbv [of_list_nat].
+      erewrite get_of_func_Some_supported; trivial; intros.
+      rewrite in_seq; split; try Lia.lia; cbn.
+      apply nth_error_Some. congruence.
+    Qed.
+
+    Lemma get_of_list_nat_at a xs i : get (of_list_nat_at a xs) (a+i) = nth_error xs i.
+    Proof.
+      cbv [of_list_nat_at].
+      rewrite get_map_keys_always_invertible, get_of_list_nat; trivial; intros; Lia.lia.
+    Qed.
+  End OfListNatAt.
+
+  Section OfListZAt.
+    Import BinInt.
+    Context {value : Type} {map : map Z value} {ok : map.ok map}.
+    Definition of_list_Z (xs : list value) : map :=
+      of_func (Znth_error xs) (List.map Z.of_nat (seq 0 (length xs))).
+    Definition of_list_Z_at (a : Z) (xs : list value) : map :=
+      map_keys (Z.add a) (of_list_Z xs).
+
+    Lemma get_of_list_Z xs i : get (of_list_Z xs) i = Znth_error xs i.
+    Proof.
+      pose proof Decidable.Z.eqb_spec.
+      cbv [Znth_error of_list_Z].
+      erewrite get_of_func_Some_supported; trivial; intros.
+      destruct (Z.ltb_spec k 0%Z) in *; try discriminate.
+      eapply in_map_iff; exists (Z.to_nat k); rewrite ?in_seq;
+        repeat split; rewrite ?Znat.Z2Nat.id; try Lia.lia; cbn.
+      apply nth_error_Some. congruence.
+    Qed.
+
+    Lemma get_of_list_Z_at a xs i : get (of_list_Z_at a xs) i = Znth_error xs (i-a)%Z.
+    Proof.
+      cbv [of_list_Z_at].
+      replace i with (a+(i-a))%Z by Lia.lia.
+      rewrite get_map_keys_always_invertible, get_of_list_Z by (intros; Lia.lia).
+      f_equal; Lia.lia.
+    Qed.
+  End OfListZAt.
+End map.
